pulse/lib/steel/pulse/Pulse.Checker.STApp.fst
@@ -7,8 +7,11 @@ open Pulse.Syntax
 open Pulse.Typing
 open Pulse.Checker.Pure
 open Pulse.Checker.Common
+open Pulse.Prover
 module RU = Pulse.RuntimeUtils
 module P = Pulse.Syntax.Printer
+
+module Prover = Pulse.Prover
 
 module FV = Pulse.Typing.FV
 let debug_log (g:env) (f:unit -> T.Tac unit) : T.Tac unit = if RU.debug_at_level (fstar_env g) "st_app" then f () else ()
@@ -33,6 +36,9 @@ let canonicalize_st_typing (#g:env) (#t:st_term) (#c:comp_st) (d:st_typing g t c
     in
     T_Equiv _ _ _ _ d st_eq
 
+let coerce_eq (#a #b:Type) (x:a) (_:squash (a === b)) : y:b { y == x } = x
+
+#push-options "--z3rlimit_factor 4 --fuel 1 --ifuel 1"
 let check_st_app
   (g:env)
   (t:st_term { Tm_STApp? t.term })
@@ -75,7 +81,7 @@ let check_st_app
         let c = (canon_comp (open_comp_with comp_typ arg)) in
         let d : st_typing g t c = d in
 
-        admit ()
+        repack (try_frame_pre ctxt_typing d) post_hint t.range
        | _ ->
          fail g (Some t.range) "Expected an effectful application; got a pure term (could it be partially applied by mistake?)"
      else fail g (Some t.range) (Printf.sprintf "Unexpected qualifier in head type %s of stateful application: head = %s, arg = %s"
@@ -84,97 +90,97 @@ let check_st_app
                  (P.term_to_string arg))
 
   | _ -> fail g (Some t.range) (Printf.sprintf "Unexpected head type in impure application: %s" (P.term_to_string ty_head))
-
-
-#push-options "--fuel 0 --ifuel 1 --z3rlimit_factor 2"
-let check_stapp
-  (allow_inst:bool)
-  (g:env)
-  (t:st_term{Tm_STApp? t.term})
-  (pre:term)
-  (pre_typing:tot_typing g pre tm_vprop)
-  (post_hint:post_hint_opt g)
-  (frame_pre:bool)
-  (check':bool -> check_t)
-  : T.Tac (checker_result_t g pre post_hint frame_pre) =
-  // maybe_log t;
-  let range = t.range in
-  let Tm_STApp { head; arg_qual=qual; arg } = t.term in
-
-  //
-  // c is the comp remaining after applying head to arg,
-  //
-  // let infer_logical_implicits_and_check
-  //   (t:term)
-  //   (c:comp{C_Tot? c}) : T.Tac _ =
-
-  //   match c with
-  //   | C_Tot ty ->
-  //     begin match is_arrow ty with
-  //           | Some (_, Some Implicit, _) -> 
-  //             //Some implicits to follow
-  //             let t = Pulse.Checker.Inference.infer g t ty pre range in
-  //             check' false g t pre pre_typing post_hint
-  //           | _ ->
-  //             T.fail "Unexpected c in infer_logical_implicits_and_check"
-  //     end
-
-  //   | _ ->
-  //     T.fail "Unexpected c in infer_logical_implicits_and_check" in
-
-  let check_st_app ()  : T.Tac (checker_result_t g pre post_hint frame_pre) =
-    let g = push_context "st_app" t.range g in        
-    let (| head, ty_head, dhead |) = check_term g head in
-    debug_log g (fun _ ->
-        T.print (Printf.sprintf "st_app: head = %s, ty_head = %s\n"
-                   (P.term_to_string head)
-                   (P.term_to_string ty_head)));
-    match is_arrow ty_head with
-    | Some ({binder_ty=formal;binder_ppname=ppname}, bqual, comp_typ) ->
-        is_arrow_tm_arrow ty_head;
-        debug_log g (fun _ ->
-         T.print (Printf.sprintf "st_app, readback comp as %s\n"
-                   (P.comp_to_string comp_typ)));
-    
-        assert (ty_head ==
-                tm_arrow ({binder_ty=formal;binder_ppname=ppname}) bqual comp_typ);
-        if qual = bqual
-        then
-         let (| arg, darg |) = check_term_with_expected_type g arg formal in
-         match comp_typ with
-         | C_ST res
-         | C_STAtomic _ res
-         | C_STGhost _ res ->
-           // This is a real ST application
-           let d : st_typing _ _ (open_comp_with comp_typ arg) = T_STApp g head formal qual comp_typ arg (E dhead) (E darg) in
-           let d' = canonicalize_st_typing d in
-          //  T.print (Printf.sprintf "ST application trying to frame, context: %s and pre: %s\n"
-          //             (Pulse.Syntax.Printer.term_to_string pre)
-          //             (Pulse.Syntax.Printer.term_to_string (comp_pre (open_comp_with comp_typ arg))));
-          if frame_pre
-          then repack (try_frame_pre pre_typing d') post_hint
-          else if Some? post_hint
-          then T.fail "stapp: frame_pre is false but post_hint is set, bailing"
-          else (| _, _, d' |)
-         | _ ->
-           fail g (Some t.range) "Expected an effectful application; got a pure term (could it be partially applied by mistake?)"
-        else 
-         fail g (Some t.range) (Printf.sprintf "Unexpected qualifier in head type %s of stateful application: head = %s, arg = %s"
-                                  (P.term_to_string ty_head)
-                                  (P.term_to_string head)
-                                  (P.term_to_string arg))
-    
-     | _ -> fail g (Some t.range) (Printf.sprintf "Unexpected head type in impure application: %s" (P.term_to_string ty_head))
-  in
-
-  let g = push_context "pure_app" t.range g in    
-  let pure_app = tm_pureapp head qual arg in
-  let t, ty = instantiate_term_implicits g pure_app in
-  match is_arrow ty with
-  | Some (_, Some Implicit, _) -> 
-    //Some implicits to follow
-    let t = Pulse.Checker.Inference.infer g t ty pre range in
-    check' false g t pre pre_typing post_hint frame_pre
-  | _ ->
-    check_st_app ()
 #pop-options
+
+// #push-options "--fuel 0 --ifuel 1 --z3rlimit_factor 2"
+// let check_stapp
+//   (allow_inst:bool)
+//   (g:env)
+//   (t:st_term{Tm_STApp? t.term})
+//   (pre:term)
+//   (pre_typing:tot_typing g pre tm_vprop)
+//   (post_hint:post_hint_opt g)
+//   (frame_pre:bool)
+//   (check':bool -> check_t)
+//   : T.Tac (checker_result_t g pre post_hint frame_pre) =
+//   // maybe_log t;
+//   let range = t.range in
+//   let Tm_STApp { head; arg_qual=qual; arg } = t.term in
+
+//   //
+//   // c is the comp remaining after applying head to arg,
+//   //
+//   // let infer_logical_implicits_and_check
+//   //   (t:term)
+//   //   (c:comp{C_Tot? c}) : T.Tac _ =
+
+//   //   match c with
+//   //   | C_Tot ty ->
+//   //     begin match is_arrow ty with
+//   //           | Some (_, Some Implicit, _) -> 
+//   //             //Some implicits to follow
+//   //             let t = Pulse.Checker.Inference.infer g t ty pre range in
+//   //             check' false g t pre pre_typing post_hint
+//   //           | _ ->
+//   //             T.fail "Unexpected c in infer_logical_implicits_and_check"
+//   //     end
+
+//   //   | _ ->
+//   //     T.fail "Unexpected c in infer_logical_implicits_and_check" in
+
+//   let check_st_app ()  : T.Tac (checker_result_t g pre post_hint frame_pre) =
+//     let g = push_context "st_app" t.range g in        
+//     let (| head, ty_head, dhead |) = check_term g head in
+//     debug_log g (fun _ ->
+//         T.print (Printf.sprintf "st_app: head = %s, ty_head = %s\n"
+//                    (P.term_to_string head)
+//                    (P.term_to_string ty_head)));
+//     match is_arrow ty_head with
+//     | Some ({binder_ty=formal;binder_ppname=ppname}, bqual, comp_typ) ->
+//         is_arrow_tm_arrow ty_head;
+//         debug_log g (fun _ ->
+//          T.print (Printf.sprintf "st_app, readback comp as %s\n"
+//                    (P.comp_to_string comp_typ)));
+    
+//         assert (ty_head ==
+//                 tm_arrow ({binder_ty=formal;binder_ppname=ppname}) bqual comp_typ);
+//         if qual = bqual
+//         then
+//          let (| arg, darg |) = check_term_with_expected_type g arg formal in
+//          match comp_typ with
+//          | C_ST res
+//          | C_STAtomic _ res
+//          | C_STGhost _ res ->
+//            // This is a real ST application
+//            let d : st_typing _ _ (open_comp_with comp_typ arg) = T_STApp g head formal qual comp_typ arg (E dhead) (E darg) in
+//            let d' = canonicalize_st_typing d in
+//           //  T.print (Printf.sprintf "ST application trying to frame, context: %s and pre: %s\n"
+//           //             (Pulse.Syntax.Printer.term_to_string pre)
+//           //             (Pulse.Syntax.Printer.term_to_string (comp_pre (open_comp_with comp_typ arg))));
+//           if frame_pre
+//           then repack (try_frame_pre pre_typing d') post_hint
+//           else if Some? post_hint
+//           then T.fail "stapp: frame_pre is false but post_hint is set, bailing"
+//           else (| _, _, d' |)
+//          | _ ->
+//            fail g (Some t.range) "Expected an effectful application; got a pure term (could it be partially applied by mistake?)"
+//         else 
+//          fail g (Some t.range) (Printf.sprintf "Unexpected qualifier in head type %s of stateful application: head = %s, arg = %s"
+//                                   (P.term_to_string ty_head)
+//                                   (P.term_to_string head)
+//                                   (P.term_to_string arg))
+    
+//      | _ -> fail g (Some t.range) (Printf.sprintf "Unexpected head type in impure application: %s" (P.term_to_string ty_head))
+//   in
+
+//   let g = push_context "pure_app" t.range g in    
+//   let pure_app = tm_pureapp head qual arg in
+//   let t, ty = instantiate_term_implicits g pure_app in
+//   match is_arrow ty with
+//   | Some (_, Some Implicit, _) -> 
+//     //Some implicits to follow
+//     let t = Pulse.Checker.Inference.infer g t ty pre range in
+//     check' false g t pre pre_typing post_hint frame_pre
+//   | _ ->
+//     check_st_app ()
+// #pop-options
