pulse/lib/steel/pulse/Pulse.Prover.Substs.fst
@@ -263,6 +263,22 @@ let rec ss_to_nt_substs (g:env) (uvs:env) (ss:ss_t)
            Some nts
     else None
 
+let well_typed_nt_substs_prefix (g:env) (uvs:env) (nts:nt_substs)
+  (uvs1:env)
+  : Pure nt_substs
+         (requires well_typed_nt_substs g uvs nts /\ env_extends uvs uvs1)
+         (ensures fun nts1 -> well_typed_nt_substs g uvs1 nts1)
+         (decreases L.length nts) =
+  match bindings uvs1, bindings uvs with
+  | [], _ -> []
+  | _::_, _::_ ->
+    let x1, ty1, rest_uvs1 = remove_binding uvs1 in
+    let x, ty, rest_uvs = remove_binding uvs in
+    assume (x1 == x /\ ty1 == ty);
+    let (NT y e)::nts_rest = nts in
+    assume (env_extends (subst_env rest_uvs [ NT y e ]) (subst_env rest_uvs1 [ NT y e ]));
+    (NT y e)::(well_typed_nt_substs_prefix g (subst_env rest_uvs [ NT y e ]) nts_rest (subst_env rest_uvs1 [ NT y e ]))
+
 let ss_nt_subst (g:env) (uvs:env) (ss:ss_t) (nts:nt_substs)
   : Lemma (requires disjoint uvs g /\ well_typed_nt_substs g uvs nts /\ is_permutation nts ss)
           (ensures
