pulse/lib/steel/pulse/Pulse.Checker.STApp.fsti
@@ -7,11 +7,9 @@ open Pulse.Typing
 open Pulse.Checker.Common
 
 val check_stapp
-  (allow_inst:bool)
   (g:env)
   (t:st_term{Tm_STApp? t.term})
   (pre:term)
   (pre_typing:tot_typing g pre tm_vprop)
   (post_hint:post_hint_opt g)
-  (check':bool -> check_t)
   : T.Tac (checker_result_t g pre post_hint)
