pulse/lib/steel/pulse/Pulse.Prover.Match.fsti
@@ -4,6 +4,8 @@ module T = FStar.Tactics
 
 open Pulse.Syntax
 open Pulse.Typing
+
+open Pulse.Checker.Common
 open Pulse.Prover.Common
 
 val match_step (#preamble:preamble) (pst:prover_state preamble)
