pulse/lib/steel/pulse/Pulse.Prover.fsti
@@ -4,17 +4,29 @@ module T = FStar.Tactics.V2
 
 open Pulse.Syntax
 open Pulse.Typing
+open Pulse.Checker.Common
 open Pulse.Prover.Common
 
 module PS = Pulse.Prover.Substs
 
 val prove
-  (#g:env) (#ctxt:vprop) (ctxt_typing:vprop_typing g ctxt)
+  (#g:env) (#ctxt:vprop) (ctxt_typing:tot_typing g ctxt tm_vprop)
   (uvs:env { disjoint g uvs })
-  (#goals:vprop) (goals_typing:vprop_typing (push_env g uvs) goals)
+  (#goals:vprop) (goals_typing:tot_typing (push_env g uvs) goals tm_vprop)
 
   : T.Tac (g1 : env { g1 `env_extends` g } &
-           uvs1 : env { uvs1 `env_extends` uvs /\ disjoint uvs1 g1 } &
-           nts1 : PS.nt_substs { PS.well_typed_nt_substs g1 uvs1 nts1 } &
+           nts : PS.nt_substs { PS.well_typed_nt_substs g1 uvs nts } &
            remaining_ctxt : vprop &
-           continuation_elaborator g ctxt g1 ((PS.nt_subst_term goals nts1) * remaining_ctxt))
+           continuation_elaborator g ctxt g1 ((PS.nt_subst_term goals nts) * remaining_ctxt))
+
+val try_frame_pre (#g:env) (#ctxt:vprop) (ctxt_typing:tot_typing g ctxt tm_vprop)
+  (#t:st_term) (#c:comp_st) (d:st_typing g t c)
+
+  : T.Tac (checker_result_t g ctxt None)
+
+val repack (#g:env) (#ctxt:vprop)
+  (r:checker_result_t g ctxt None)
+  (post_hint:post_hint_opt g)
+  (rng:range)
+  
+  : T.Tac (checker_result_t g ctxt post_hint)
